Checkpoint.

MQuinnHoare.v
@@ -6,3 +6,162 @@ Require Import Coq.omega.Omega.
 Require Import MQuinnImp.
 Require Import MQuinnMaps.
 
+Definition Assertion := state -> Prop.
+
+Module ExAssertions.
+
+Definition as1 : Assertion := fun st => st X = 3.
+(* Holds for every state in which X is 3. *)
+
+Definition as2 : Assertion := fun st => st X <= st Y.
+(* Holds for every state in which X is <= Y. *)
+
+Definition as3 : Assertion :=
+  fun st => st X = 3 \/ st X <= st Y.
+(* Holds for every state in which X is 3 or X is <= Y. *)
+
+Definition as4 : Assertion :=
+  fun st => st Z * st Z <= st X /\
+            ~ (((S (st Z)) * (S (st Z))) <= st X).
+(* Holds for every state in which Z*Z is <= X
+     AND (Z+1*Z+1) is NOT <= X. *)
+
+Definition as5 : Assertion := fun st => True.
+(* Holds for every state. *)
+
+Definition as6 : Assertion := fun st => False.
+(* Does not hold for any state. *)
+
+End ExAssertions.
+
+Definition assert_implies (P Q : Assertion) : Prop :=
+  forall st, P st -> Q st.
+
+Notation "P ->> Q" := (assert_implies P Q)
+                      (at level 80) : hoare_spec_scope.
+Open Scope hoare_spec_scope.
+
+Notation "P <<->> Q" :=
+  (P ->> Q /\ Q ->> P) (at level 80) : hoare_spec_scope.
+
+Definition hoare_triple
+           (P:Assertion) (c:com) (Q:Assertion) : Prop :=
+  forall st st',
+     c / st \\ st' ->
+     P st ->
+     Q st'.
+
+Notation "{{ P }} c {{ Q }}" :=
+  (hoare_triple P c Q) (at level 90, c at next level)
+  : hoare_spec_scope.
+
+(*
+1) {{True}} c {{X = 5}}
+   If c is run in any state, it results in a state in which X is 5.
+
+2) {{X = m}} c {{X = m + 5)}}
+   If c is run in a state where X is m, it results in a state where
+   X is m + 5.
+
+3) {{X ≤ Y}} c {{Y ≤ X}}
+   If c is run in a state where X is <= Y, it results in state where
+   Y <= X.
+
+4) {{True}} c {{False}}
+   If c is run in any state, it does not result in any state.
+
+5) {{X = m}}
+   c
+   {{Y = real_fact m}}
+   If c is run in any state where X = m, it results in a state where
+   Y is (real_fact m).
+
+6) {{True}}
+   c
+   {{(Z * Z) ≤ m ∧ ¬ (((S Z) * (S Z)) ≤ m)}}
+   If c is run in any state, it results in a state where
+   (Z * Z) ≤ m ∧ ¬ (((S Z) * (S Z)) ≤ m).
+*)
+
+(*
+1) {{True}} X ::= 5 {{X = 5}}
+   VALID
+
+2) {{X = 2}} X ::= X + 1 {{X = 3}}
+   VALID
+
+3) {{True}} X ::= 5; Y ::= 0 {{X = 5}}
+   VALID
+
+4) {{X = 2 ∧ X = 3}} X ::= 5 {{X = 0}}
+   INVALID
+
+5) {{True}} SKIP {{False}}
+   INVALID
+
+6) {{False}} SKIP {{True}}
+   INVALID
+
+7) {{True}} WHILE True DO SKIP END {{False}}
+   VALID
+
+8) {{X = 0}}
+    WHILE X == 0 DO X ::= X + 1 END
+    {{X = 1}}
+    VALID
+
+9) {{X = 1}}
+    WHILE X ≠ 0 DO X ::= X + 1 END
+    {{X = 100}} 
+    INVALID
+*)
+
+Theorem hoare_post_true : forall (P Q : Assertion) c,
+  (forall st, Q st) ->
+  {{P}} c {{Q}}.
+Proof.
+  intros. unfold hoare_triple. intros. apply H.
+Qed.
+
+Theorem hoare_pre_false : forall (P Q : Assertion) c,
+  (forall st, ~(P st)) ->
+  {{P}} c {{Q}}.
+Proof.
+  intros P Q c H. unfold hoare_triple.
+  intros st st' Heval HP.
+  unfold not in H. apply H in HP.
+  inversion HP. Qed.
+
+Definition assn_sub X a P : Assertion :=
+  fun (st : state) =>
+    P (t_update st X (aeval st a)).
+
+Notation "P [ X |-> a ]" := (assn_sub X a P) (at level 10).
+
+Theorem hoare_asgn : forall Q X a,
+  {{Q [X |-> a]}} (X ::= a) {{Q}}.
+Proof.
+  unfold hoare_triple.
+  intros Q X a st st' HE HQ.
+  inversion HE. subst. unfold assn_sub in HQ. assumption.
+Qed.
+
+Example assn_sub_example :
+  {{(fun st => st X = 3) [X |-> ANum 3]}}
+  (X ::= (ANum 3))
+  {{fun st => st X = 3}}.
+Proof.
+  apply hoare_asgn. Qed.
+
+Example assn_sub_ex1 :
+  {{(fun st => st X <= 5) [X |-> APlus (AId X) (ANum 1)]}}
+  (X ::= (APlus (AId X) (ANum 1)))
+  {{(fun st => st X <= 5)}}.
+Proof. apply hoare_asgn. Qed.
+
+Example assn_sub_ex2 :
+  {{(fun st => (0 <= st X /\ st X <= 5)) [X |-> ANum 3] }}
+  (X ::= (ANum 3))
+  {{(fun st => 0 <= st X /\ st X <= 5)}}.
+Proof. apply hoare_asgn. Qed.
+
